Partially implement execution plan specification

src/ExecutionPlan.v
@@ -15,6 +15,23 @@ Require Import Maps.
 Require Import Utils.
 Import PropertyGraph.
 
+Module FilterMode.
+  Inductive t : Type :=
+  | Vertices
+  | Edges
+  .
+End FilterMode.
+
+Module ExpandMode .
+  Inductive t : Type :=
+  | All
+  | Into
+  .
+End ExpandMode.
+
+Import FilterMode.
+Import ExpandMode.
+
 Module ExecutionPlan.
   Definition step0 := PropertyGraph.t -> option BindingTable.t.
   Definition step1 := PropertyGraph.t -> BindingTable.t -> option BindingTable.t.
@@ -23,99 +40,141 @@ Module ExecutionPlan.
     (* scan_vertices (n : Pattern.name) : step0 *)
     Parameter scan_vertices : Pattern.name -> step0.
 
-    (* filter_by_label (n : Pattern.name) (l : label) : step1 *)
-    Parameter filter_by_label : Pattern.name -> label -> step1.
+    (* filter_by_label (mode : FilterMode.t) (n : Pattern.name) (l : label) : step1 *)
+    Parameter filter_by_label : FilterMode.t -> Pattern.name -> label -> step1.
 
-    (* expand_all (n_from n_edge n_to : Pattern.name) (d : Pattern.direction) : step1 *)
-    Parameter expand_all : Pattern.name -> Pattern.name -> Pattern.name -> Pattern.direction -> step1.
+    (* expand (mode : ExpandMode.t) (n_from n_edge n_to : Pattern.name) (d : Pattern.direction) : step1 *)
+    Parameter expand : ExpandMode.t -> Pattern.name -> Pattern.name -> Pattern.name -> Pattern.direction -> step1.
 
-    (* expand_into (n_from n_edge n_to : Pattern.name) (d : Pattern.direction) : step1 *)
-    Parameter expand_into : Pattern.name -> Pattern.name -> Pattern.name -> Pattern.direction -> step1.
+    Section axioms.
+      Variable graph : PropertyGraph.t.
+      Variable table : BindingTable.t.
+      Variable table' : BindingTable.t.
+      Variable ty : BindingTable.T.
+
+      (** If the inputs are well-formed then the operation will return the result *)
+
+      Axiom scan_vertices_wf : forall n,
+        PropertyGraph.wf graph ->
+          exists table', scan_vertices n graph = Some table'.
+
+      Axiom filter_vertices_by_label_wf : forall n l,
+        PropertyGraph.wf graph -> BindingTable.of_type table ty ->
+          ty n = Some Value.GVertexT ->
+            exists table', filter_by_label Vertices n l graph table = Some table'.
+
+      Axiom filter_edges_by_label_wf : forall n l,
+        PropertyGraph.wf graph -> BindingTable.of_type table ty ->
+          ty n = Some Value.GEdgeT ->
+            exists table', filter_by_label Edges n l graph table = Some table'.
+
+      Axiom expand_all_wf : forall n_from n_edge n_to d,
+        PropertyGraph.wf graph -> BindingTable.of_type table ty ->
+          ty n_from = Some Value.GVertexT -> ty n_edge = None -> ty n_to = None ->
+              exists table', expand All n_from n_edge n_to d graph table = Some table'.
+      
+      Axiom expand_into_wf : forall n_from n_edge n_to d,
+        PropertyGraph.wf graph -> BindingTable.of_type table ty ->
+          ty n_from = Some Value.GVertexT -> ty n_edge = None -> ty n_to = Some Value.GVertexT ->
+            exists table', expand Into n_from n_edge n_to d graph table = Some table'.
 
 
-    (** If the inputs are well-formed then the operation will return the result *)
+      (** If the operation returned some table then the type of the table is correct *)
 
-    Axiom scan_vertices_wf : forall n graph,
-      PropertyGraph.wf graph ->
-        exists table', scan_vertices n graph = Some table'.
+      Axiom scan_vertices_type : forall n,
+        scan_vertices n graph = Some table' ->
+          BindingTable.of_type table' (n |-> Value.GVertexT).
+      
+      Axiom filter_by_label_type : forall mode n l,
+        filter_by_label mode n l graph table = Some table' ->
+          BindingTable.of_type table ty ->
+            BindingTable.of_type table' ty.
 
-    Axiom filter_by_label_wf : forall n l graph table ty,
-      PropertyGraph.wf graph -> BindingTable.of_type table ty ->
-        (ty n = Some Value.GVertexT \/ ty n = Some Value.GEdgeT) ->
-          exists table', filter_by_label n l graph table = Some table'.
+      Axiom expand_all_type : forall n_from n_edge n_to d,
+        expand All n_from n_edge n_to d graph table = Some table' ->
+          BindingTable.of_type table ty ->
+            BindingTable.of_type table'
+              (n_edge |-> Value.GEdgeT; n_to |-> Value.GVertexT; ty).
 
-    Axiom expand_all_wf : forall n_from n_edge n_to d graph table ty,
-      PropertyGraph.wf graph -> BindingTable.of_type table ty ->
-        ty n_from = Some Value.GVertexT -> ty n_edge = None -> ty n_to = None ->
-            exists table', expand_all n_from n_edge n_to d graph table = Some table'.
-    
-    Axiom expand_into_wf : forall n_from n_edge n_to d graph table ty,
-      PropertyGraph.wf graph -> BindingTable.of_type table ty ->
-        ty n_from = Some Value.GVertexT -> ty n_edge = None -> ty n_to = Some Value.GVertexT ->
-          exists table', expand_into n_from n_edge n_to d graph table = Some table'.
+      Axiom expand_into_type : forall n_from n_edge n_to d,
+        expand Into n_from n_edge n_to d graph table = Some table' ->
+          BindingTable.of_type table ty ->
+            BindingTable.of_type table'
+              (n_edge |-> Value.GEdgeT; ty).
 
+      (** scan_vertices specification *)
 
-    (** If the operation returned some table then the type of the table is correct *)
+      Axiom scan_vertices_spec : forall n v,
+        scan_vertices n graph = Some table' ->
+          (exists r, In r table' /\ r n = Some (Value.GVertex v)) <->
+              In v (vertices graph).
 
-    Axiom scan_vertices_type : forall n graph table',
-      scan_vertices n graph = Some table' ->
-        BindingTable.of_type table' (n |-> Value.GVertexT).
-    
-    Axiom filter_by_label_type : forall n l graph table table' ty,
-      filter_by_label n l graph table = Some table' ->
-        BindingTable.of_type table ty ->
-          BindingTable.of_type table' ty.
+      (** filter_by_label specification *)
 
-    Axiom expand_all_type : forall n_from n_edge n_to d graph table table' ty,
-      expand_all n_from n_edge n_to d graph table = Some table' ->
-        BindingTable.of_type table ty ->
-          BindingTable.of_type table'
-            (n_edge |-> Value.GEdgeT; n_to |-> Value.GVertexT; ty).
+      Axiom filter_vertices_by_label_spec : forall n l v r,
+        filter_by_label Vertices n l graph table = Some table' ->
+          In l (vlabels graph v) -> In r table -> r n = Some (Value.GVertex v) ->
+            (exists r', In r' table' /\ r' n = Some (Value.GVertex v)).
 
-    Axiom expand_into_type : forall n_from n_edge n_to d graph table table' ty,
-      expand_into n_from n_edge n_to d graph table = Some table' ->
-        BindingTable.of_type table ty ->
-          BindingTable.of_type table'
-            (n_edge |-> Value.GEdgeT; ty).
+      Axiom filter_vertices_by_label_spec' : forall n l v r',
+        filter_by_label Edges n l graph table = Some table' ->
+          In r' table' -> r' n = Some (Value.GVertex v) ->
+            In l (vlabels graph v) /\ exists r, In r table /\ r n = Some (Value.GVertex v).
+
+      Axiom filter_edges_by_label_spec : forall n l e r,
+        filter_by_label Edges n l graph table = Some table' ->
+          In r table -> elabel graph e = l -> r n = Some (Value.GEdge e) ->
+            (exists r', In r' table' /\ r' n = Some (Value.GEdge e)).
+
+      Axiom filter_edges_by_label_spec' : forall n l e r',
+        filter_by_label Edges n l graph table = Some table' ->
+          In r' table' -> r' n = Some (Value.GEdge e) ->
+            elabel graph e = l /\ exists r, In r table /\ r n = Some (Value.GEdge e).
+
+      (** expand_all specification *)
+
+    End axioms.
   End Spec.
 
   Inductive t :=
   | ScanVertices (n : Pattern.name)
-  | FilterByLabel (plan : t) (n : Pattern.name) (l : label)
-  | ExpandAll (plan : t) (n_from n_edge n_to : Pattern.name) (d : Pattern.direction)
-  | ExpandInto (plan : t) (n_from n_edge n_to : Pattern.name) (d : Pattern.direction)
+  | FilterByLabel (mode : FilterMode.t) (n : Pattern.name) (l : label) (plan : t) 
+  | Expand (mode : ExpandMode.t) (n_from n_edge n_to : Pattern.name) (d : Pattern.direction) (plan : t)
   .
 
   Fixpoint dom (plan : t) : list Pattern.name := 
     match plan with
     | ScanVertices n => [ n ]
-    | FilterByLabel plan n l => dom plan
-    | ExpandAll plan n_from n_edge n_to d => n_edge :: n_to :: dom plan
-    | ExpandInto plan n_from n_edge n_to d => n_edge :: dom plan
+    | FilterByLabel mode n l plan => dom plan
+    | Expand All n_from n_edge n_to d plan => n_edge :: n_to :: dom plan
+    | Expand Into n_from n_edge n_to d plan => n_edge :: dom plan
     end.
 
   Fixpoint type_of (plan : t) : BindingTable.T :=
     match plan with
     | ScanVertices n => n |-> Value.GVertexT
-    | FilterByLabel plan n l => type_of plan
-    | ExpandAll plan n_from n_edge n_to d => n_edge |-> Value.GEdgeT; n_to |-> Value.GVertexT; type_of plan
-    | ExpandInto plan n_from n_edge n_to d => n_edge |-> Value.GEdgeT; type_of plan
+    | FilterByLabel mode n l plan => type_of plan
+    | Expand All n_from n_edge n_to d plan => n_edge |-> Value.GEdgeT; n_to |-> Value.GVertexT; type_of plan
+    | Expand Into n_from n_edge n_to d plan => n_edge |-> Value.GEdgeT; type_of plan
     end.
 
   Fixpoint wf (plan : t) :=
     match plan with
     | ScanVertices n => True
-    | FilterByLabel plan n l =>
+    | FilterByLabel Vertices n l plan =>
       << Htype : type_of plan n = Some Value.GVertexT >> /\
       << Hwf : wf plan >>
-    | ExpandAll plan n_from n_edge n_to d =>
+    | FilterByLabel Edges n l plan =>
+      << Htype : type_of plan n = Some Value.GEdgeT >> /\
+      << Hwf : wf plan >>
+    | Expand All n_from n_edge n_to d plan =>
       << Htype_from : type_of plan n_from = Some Value.GVertexT >> /\
       << Htype_edge : type_of plan n_edge = None >> /\
       << Htype_to : type_of plan n_to = None >> /\
       << Hneq_from : n_from =/= n_edge >> /\
       << Hneq_to : n_to =/= n_edge >> /\
       << Hwf : wf plan >>
-    | ExpandInto plan n_from n_edge n_to d =>
+    | Expand Into n_from n_edge n_to d plan =>
       << Htype_from : type_of plan n_from = Some Value.GVertexT >> /\
       << Htype_edge : type_of plan n_edge = None >> /\
       << Htype_to : type_of plan n_to = Some Value.GVertexT >> /\
@@ -123,36 +182,6 @@ Module ExecutionPlan.
       << Hneq_to : n_to =/= n_edge >> /\
       << Hwf : wf plan >>
     end.
-
-  (* Domain of the plan is the domain of resulting binding table *)
-  Lemma dom__type_of (plan : t) (Hwf : wf plan) (n : Pattern.name) :
-    In n (dom plan) <-> exists ty, type_of plan n = Some ty.
-  Proof.
-    induction plan; simpl in *.
-    2: now apply IHplan.
-    all: split; intros H; desf.
-    - subst. rewrite update_eq. now exists (Value.GVertexT).
-    - unfold update, t_update, Pattern.name in *.
-      destruct (equiv_decbP n0 n); try discriminate H.
-      now left.
-    - rewrite update_eq. now exists (Value.GEdgeT).
-    - rewrite update_neq; [| now symmetry ].
-      rewrite update_eq. now exists (Value.GVertexT).
-    - rewrite update_neq. rewrite update_neq.
-      { now apply IHplan. }
-      all: intros ?; rewrite IHplan in H; [| now assumption ]; desf.
-    - unfold update, t_update, Pattern.name in *.
-      destruct (equiv_decbP n_edge n), (equiv_decbP n_to n); subst; auto.
-      right. right. apply IHplan; [ assumption | now exists ty ].
-      - rewrite update_eq. now exists (Value.GEdgeT).
-      - rewrite update_neq.
-        { now apply IHplan. }
-        intros ?; rewrite IHplan in H; [| now assumption ]; desf.
-      - unfold update, t_update, Pattern.name in *.
-        destruct (equiv_decbP n_edge n); subst; auto.
-        right. apply IHplan; [ assumption | now exists ty ].
-  Qed.
-      
 
   Module EvalPlan (S : Spec).
     Import S.
@@ -162,12 +191,10 @@ Module ExecutionPlan.
       Fixpoint eval (plan : ExecutionPlan.t) :=
         match plan with
         | ScanVertices n => scan_vertices n graph
-        | FilterByLabel plan n l =>
-          eval plan >>= filter_by_label n l graph
-        | ExpandAll plan n_from n_edge n_to d => 
-          eval plan >>= expand_all n_from n_edge n_to d graph
-        | ExpandInto plan n_from n_edge n_to d => 
-          eval plan >>= expand_into n_from n_edge n_to d graph
+        | FilterByLabel mode n l plan =>
+          eval plan >>= filter_by_label mode n l graph
+        | Expand mode n_from n_edge n_to d plan => 
+          eval plan >>= expand mode n_from n_edge n_to d graph
         end.
     End eval.
 
@@ -176,12 +203,14 @@ Module ExecutionPlan.
         BindingTable.of_type table' (type_of plan).
     Proof.
       generalize dependent table'.
-      induction plan; intros table' Heval; simpl in *.
+      induction plan; intros; simpl in *.
       { apply scan_vertices_type with graph. assumption. }
-      all: destruct (eval graph plan) as [table |]; try discriminate Heval.
-      - apply filter_by_label_type with n l graph table; auto.
-      - apply expand_all_type with n_from d graph table; auto.
-      - apply expand_into_type with n_from n_to d graph table; auto.
+      all: destruct (eval graph plan); try discriminate.
+
+      2: destruct mode.
+      - eapply filter_by_label_type; eauto.
+      - eapply expand_all_type; eauto.
+      - eapply expand_into_type; eauto.
     Qed.
 
     Lemma type_of_types plan k :
@@ -191,43 +220,81 @@ Module ExecutionPlan.
     Proof.
       induction plan; simpl in *.
       all: try unfold update, t_update, Pattern.name in *.
-      all: try (destruct (n ==b k)).
-      all: try (destruct (n_edge ==b k)).
-      all: try (destruct (n_to ==b k)).
+      all: desf.
       all: auto.
     Qed.
 
     Theorem eval_wf plan graph (Hwf : wf plan) (Hwf' : PropertyGraph.wf graph) :
         exists table', eval graph plan = Some table'.
-    Proof.
-      induction plan. all: simpl in *; desf.
-      { apply scan_vertices_wf. assumption. }
+    Proof with (try eassumption).
+      induction plan. all: simpl in *; desf; desf.
+      { apply scan_vertices_wf... }
       all: destruct IHplan as [table IH]; [ now assumption | ].
       all: rewrite IH.
-      { 
-        apply filter_by_label_wf with (type_of plan); try assumption. 
-        - apply eval_type_of in IH. assumption.
-        - assert (H' := type_of_types plan n). desf. auto.
-      }
-      1: apply expand_all_wf with (type_of plan); try assumption.
-      2: apply expand_into_wf with (type_of plan); try assumption.
-      all: apply eval_type_of in IH; assumption.
+      1: eapply filter_vertices_by_label_wf...
+      2: eapply filter_edges_by_label_wf...
+      3: eapply expand_all_wf...
+      4: eapply expand_into_wf...
+      all: eapply eval_type_of...
     Qed.
   End EvalPlan.
 End ExecutionPlan.
 
 Module ExecutionPlanImpl : ExecutionPlan.Spec.
+
   Definition scan_vertices (n : Pattern.name)
                         (graph : PropertyGraph.t)
                         : option BindingTable.t :=
     Some (map (fun v => n |-> Value.GVertex v) (vertices graph)).
 
-  Definition filter_by_label (n : Pattern.name)
+  Section filter_vertices_by_label.
+    Variable n : Pattern.name.
+    Variable l : PropertyGraph.label.
+    Variable graph : PropertyGraph.t.
+
+    Fixpoint filter_vertices_by_label (table : BindingTable.t)
+      : option BindingTable.t :=
+      match table with
+      | nil => Some nil
+      | r :: table =>
+        match r n, filter_vertices_by_label table with
+        | Some (Value.GVertex v), Some table' =>
+            if In_dec l (vlabels graph v)
+            then Some (r :: table') else Some table'
+        | _, _ => None
+        end
+      end.
+  End filter_vertices_by_label.
+
+  Section filter_edges_by_label.
+    Variable n : Pattern.name.
+    Variable l : PropertyGraph.label.
+    Variable graph : PropertyGraph.t.
+
+    Fixpoint filter_edges_by_label (table : BindingTable.t)
+      : option BindingTable.t :=
+      match table with
+      | nil => Some nil
+      | r :: table =>
+        match r n, filter_edges_by_label table with
+        | Some (Value.GEdge e), Some table' =>
+            if elabel graph e == l
+            then Some (r :: table') else Some table'
+        | _, _ => None
+        end
+      end.
+  End filter_edges_by_label.
+
+  Definition filter_by_label (mode : FilterMode.t)
+                             (n : Pattern.name)
                              (l : PropertyGraph.label)
                              (graph : PropertyGraph.t)
                              (table : BindingTable.t)
-                             : option BindingTable.t.
-  Admitted.
+                             : option BindingTable.t :=
+    match mode with
+    | Vertices => filter_vertices_by_label n l graph table
+    | Edges => filter_edges_by_label n l graph table
+    end.
 
   Definition expand_all (n_from n_edge n_to : Pattern.name)
                         (d : Pattern.direction)
@@ -242,5 +309,182 @@ Module ExecutionPlanImpl : ExecutionPlan.Spec.
                          (table : BindingTable.t)
                          : option BindingTable.t :=
     expand_all n_from n_edge n_to d graph table.
+
+  Definition expand (mode : ExpandMode.t)
+                    (n_from n_edge n_to : Pattern.name)
+                    (d : Pattern.direction)
+                    (graph : PropertyGraph.t)
+                    (table : BindingTable.t)
+                    : option BindingTable.t :=
+    match mode with
+    | All => expand_all n_from n_edge n_to d graph table
+    | Into => expand_into n_from n_edge n_to d graph table
+    end.
+
+  (** If the inputs are well-formed then the operation will return the result *)
+
+  Lemma scan_vertices_wf graph n (Hwf : PropertyGraph.wf graph) :
+    exists table', scan_vertices n graph = Some table'.
+  Proof.
+    now eexists.
+  Qed.
+
+  Lemma filter_vertices_by_label_wf graph table ty n l
+                                    (Hwf : PropertyGraph.wf graph)
+                                    (Htype : BindingTable.of_type table ty)
+                                    (Hty : ty n = Some Value.GVertexT) :
+    exists table', filter_vertices_by_label n l graph table = Some table'.
+  Proof.
+    induction table as [| r table IH]; simpl in *.
+    { now eexists. }
+    assert (exists v, r n = Some (Value.GVertex v)) as [v Hval];
+      [ apply Rcd.type_of_GVertexT; rewrite Htype; [assumption | now left ] | ].
+    rewrite Hval.
+    destruct IH as [table' IH]; eauto.
+    rewrite IH. desf.
+    all: now eexists.
+  Qed.
+
+  Lemma filter_edges_by_label_wf graph table ty n l
+                                 (Hwf : PropertyGraph.wf graph)
+                                 (Htype : BindingTable.of_type table ty)
+                                 (Hty : ty n = Some Value.GEdgeT) :
+    exists table', filter_edges_by_label n l graph table = Some table'.
+  Proof.
+    induction table as [| r table IH]; simpl in *.
+    { now eexists. }
+    assert (exists e, r n = Some (Value.GEdge e)) as [e Hval];
+      [ apply Rcd.type_of_GEdgeT; rewrite Htype; [assumption | now left ] | ].
+    rewrite Hval.
+    destruct IH as [table' IH]; eauto.
+    rewrite IH. desf.
+    all: now eexists.
+  Qed.
+
+  (** If the operation returned some table then the type of the table is correct *)
+
+  Lemma scan_vertices_type graph table' n 
+                           (Hres : scan_vertices n graph = Some table') :
+    BindingTable.of_type table' (n |-> Value.GVertexT).
+  Proof.
+    unfold scan_vertices in Hres.
+    unfold update, t_update, Pattern.name, equiv_decb,
+           BindingTable.of_type, Rcd.type_of in *.
+
+    injection Hres as Hres. subst. intros r' HIn.
+    apply in_map_iff in HIn as [r [Heq HIn]].
+    subst. extensionality k.
+    desf.
+  Qed.
+  
+  Lemma filter_by_label_type graph table table' ty mode n l
+                             (Hres : filter_by_label mode n l graph table = Some table')
+                             (Htype : BindingTable.of_type table ty) :
+    BindingTable.of_type table' ty.
+  Proof.
+    generalize dependent table'.
+    destruct mode.
+    all: induction table as [| r table IH]; simpl in *;
+          intros table' Hres; desf.
+    all: try injection Hres; ins.
+    all: eauto.
+  Qed.
+
+  (** scan_vertices specification *)
+
+  Definition scan_vertices_spec graph table' n v 
+                                (Hres : scan_vertices n graph = Some table') :
+    (exists r, In r table' /\ r n = Some (Value.GVertex v)) <->
+      In v (vertices graph).
+  Proof.
+    injection Hres as Hres. subst.
+    split.
+    - intros [r [HIn Hval]].
+      apply in_map_iff in HIn as [v' [Heq HIn]]. subst.
+      rewrite update_eq in Hval. injection Hval as Hval.
+      now subst.
+    - intros HIn. eexists. split.
+      apply in_map. { now eassumption. }
+      apply update_eq.
+  Qed.
+
+  (** filter_by_label specification *)
+
+  Lemma filter_vertices_by_label_spec graph table table' n l v r 
+                                      (Hres : filter_by_label Vertices n l graph table = Some table')
+                                      (HIn_l : In l (vlabels graph v)) (HIn : In r table)
+                                      (Hval : r n = Some (Value.GVertex v)) :
+    exists r', In r' table' /\ r' n = Some (Value.GVertex v).
+  Proof.
+    generalize dependent table'.
+    all: induction table as [| r0 table IH];
+           simpls; intros table' Hres; desf.
+
+    (* r = r0 *)
+    { exists r. split; [now left | assumption]. }
+
+    (* r <> r0 *)
+    all: edestruct IH as [r' [HIn' Hval']]; eauto.
+    all: eexists; split; [ right; eassumption | assumption ].
+  Qed.
+
+  Lemma filter_edges_by_label_spec graph table table' n l e r 
+                                   (Hres : filter_by_label Edges n l graph table = Some table')
+                                   (HIn_l : elabel graph e = l) (HIn : In r table)
+                                   (Hval : r n = Some (Value.GEdge e)) :
+    exists r', In r' table' /\ r' n = Some (Value.GEdge e).
+  Proof.
+    generalize dependent table'.
+    all: induction table as [| r0 table IH];
+           simpl in *; intros table' Hres; desf.
+
+    (* r = r0 *)
+    { exists r. split; [now left | assumption]. }
+
+    (* r <> r0 *)
+    all: edestruct IH as [r' [HIn' Hval']]; eauto.
+    all: eexists; split; [ right; eassumption | assumption ].
+  Qed.
+
+  Lemma filter_by_label_spec_v' graph table table' n l v r'
+                               (Hres : filter_by_label n l graph table = Some table')
+                               (HIn' : In r' table')
+                               (Hval' : r' n = Some (Value.GVertex v)) :
+    In l (vlabels graph v) /\ exists r, In r table /\ r n = Some (Value.GVertex v).
+  Proof.
+    generalize dependent table'.
+    induction table as [| r0 table IH];
+      simpl in *; intros table' Hres; desf.
+    all: split; try assumption.
+    all: unfold equiv in *; subst.
+
+    (* Solve goals of the form (In l _) *)
+    all: try match goal with
+             |- In _ _ =>
+                try destruct HIn';
+                try subst; try congruence;
+                edestruct IH; auto
+             end.
+
+    { destruct HIn'; subst. exists r'.
+      - split; [now left | assumption].
+      - edestruct IH as [? [? [? ?]]]; auto. eexists.
+       split; [right; eassumption | assumption]. }
+    all: try destruct HIn'; subst.
+    all: try congruence.
+    all: try edestruct IH as [? [? [? ?]]]; auto.
+    all: eexists; split; auto.
+    2: {}
+
+    (* r <> r0 *)
+    all: edestruct IH as [r' [HIn' Hval']]; eauto.
+    all: eexists; split; [ right; eassumption | assumption ].
+  Qed.
+(* 
+  Lemma filter_by_label_spec_e graph table table' n l e
+                               (Hres : filter_by_label n l graph table = Some table') :
+      (exists r', In r' table' /\ r' n = Some (Value.GEdge e)) <->
+        (exists r, In r table /\ r n = Some (Value.GEdge e)) /\ elabel graph e = l.
+  Admitted. *)
 End ExecutionPlanImpl.
 
