src/Utils.v
@@ -3,21 +3,10 @@ Require Import String.
 Require Import List.
 Require Import Bool.
 Require Import BinNums.
+From hahn Require Import HahnBase.
 From Coq Require Export Classes.EquivDec.
 From Coq Require Export Classes.RelationClasses.
 Import ListNotations.
-
-Fixpoint list_inb {A : Type} `{EqDec A eq} (e : A) (l : list A) : bool :=
-  match l with 
-  | [] => false 
-  | h :: tl => if (e ==b h) then true else list_inb e tl
-  end.
-
-Fixpoint list_inb_b (e : bool) (l : list bool) : bool :=
-  match l with 
-  | [] => false 
-  | h :: tl => if (Bool.eqb e h) then true else list_inb_b e tl
-  end.
 
 Definition option_bind {A B : Type} (x : option A) (f : A -> option B) : option B :=
   match x with
@@ -88,3 +77,83 @@ Proof.
   intros x y Hneq Heq.
   apply Hneq. symmetry. apply Heq.
 Qed.
+
+Fixpoint In_dec {A : Type} `{EqDec A eq} (a : A) (xs : list A) : {In a xs} + {~ In a xs}.
+  refine (match xs with
+          | nil => right _
+          | x :: xs => if (a == x) then left _ else
+            match In_dec _ _ _ a xs with
+            | left p => left _
+            | right np => right _
+            end
+          end).
+  all: unfold equiv, complement in *.
+  all: simpl in *; subst.
+  all: auto.
+  intros contra. desf.
+Defined.
+
+Fixpoint fold_option {A : Type} (xs : list (option A)) : option (list A) :=
+  match xs with
+  | nil => Some nil
+  | x :: xs => x >>= fun x' => fold_option xs >>= fun xs' => Some (x' :: xs')
+  end.
+
+Lemma fold_option_some {A : Type} (xs : list (option A))
+                       (Hsome : forall a, In a xs -> exists a', a = Some a') :
+  exists xs', fold_option xs = Some xs'.
+Proof.
+  induction xs as [| x xs]. { now eexists. }
+
+  destruct Hsome with x. { now left. }
+  destruct IHxs as [? IHxs]. { intros. apply Hsome. now right. }
+
+  subst. simpl. rewrite IHxs. simpl. now eexists.
+Qed.
+
+Lemma fold_option_In {A : Type} (xs : list (option A)) (xs' : list A) (a' : A) 
+                     (H : fold_option xs = Some xs') :
+  In (Some a') xs <-> In a' xs'.
+Proof.
+  generalize dependent xs'.
+  induction xs as [| x xs]; intros xs'.
+  - simpl. split.
+    2: injection H as H; subst.
+    all: contradiction.
+  - intros H. simpl. split.
+    all: destruct xs' as [|x' xs'].
+    3: contradiction.
+    all: intros [Hx | Hx]; subst.
+    all: try destruct x as [a |]; simpl in H;
+         destruct (fold_option xs); simpl in *.
+    all: try discriminate.
+    all: injection H; intros; subst.
+    1, 3: now left.
+    all: right; eapply IHxs; eauto.
+Qed.
+
+Lemma fold_option_none {A : Type} (xs : list (option A))
+                       (Hnone : In None xs) :
+  fold_option xs = None.
+Proof.
+  induction xs as [| x xs], Hnone.
+  - now subst.
+  - simpl. rewrite (IHxs H). now destruct x.
+Qed.
+
+Section filter_map.
+  Variable A B : Type.
+  Variable f : A -> option B.
+
+  Fixpoint filter_map (xs : list A) : list B :=
+    match xs with
+    | nil => nil
+    | x :: xs =>
+      match f x with
+      | Some y => y :: filter_map xs
+      | None => filter_map xs
+      end
+    end.
+End filter_map.
+
+Arguments filter_map {A B} f xs.
